lockserver/proof.dfy
@@ -26,7 +26,7 @@ lemma Inv_Next(cons:Constants, ds:DistrSys, ds':DistrSys)
     ensures Inv(cons, ds')
 {
     // TODO
-    lemma_Inv_Next_Trivialities(cons, ds, ds);
+    lemma_Inv_Next_Trivialities(cons, ds, ds');
     assume false;
 }
 
@@ -35,6 +35,12 @@ lemma lemma_Inv_Next_Trivialities(cons:Constants, ds:DistrSys, ds':DistrSys)
     requires Next(cons, ds, ds')
     ensures Trivialities(cons, ds')
 {
+    assert ds'.WF(cons);
+
+    // First prove ValidPackets(cons, ds')
+
+
+
 
 }
 
